\newcommand{\graysum}[1]{\sum\textcolor{lightgray}{#1}}

%\newcommand{\IN}{\sum_{i=1}^n}
\newcommand{\IN}{\graysum{_{i=1}^n}}
\newcommand{\geo}{\graysum{_{i=0}^n}}
\newcommand{\INzwei}{\sum_{i=2}^n}
\newcommand{\mathitem}[1]{\item$ #1 $}

\newcommand{\gn}{\textcolor{blue}{g(n)}}
\newcommand{\fn}{\textcolor{magenta}{f(n)}}



\minpurp{O-Notation}
$\gn = O(\fn) \Leftrightarrow \left(\gn\frac{1}{\fn}\right)$ ist beschraenkt (z.B. Konvergent)\\
Fester Wert => g =O(f(n)) UND f = O(g(n);

\minmeth{Logarithmen}
\begin{minipage}[t]{0.25\textwidth}
\begin{itemize}
\item $log(xy) = log(x) + log(y)$
\item $log(x^c) = clog(x)$
\end{itemize}
\end{minipage}
\begin{minipage}[t]{0.25\textwidth}
\begin{itemize}
\item $e^{ln(x)} = x$
\item ${ln(e^x)} = x$
\end{itemize}
\end{minipage}


\minpurp{Differenzengleichungen}
\halfpage{\begin{enumerate}
\item Aus Angabe lesen:\\   \textcolor{blue}{b}: Für Eingabe=1,  ~~~~~
$ x_n = \textcolor{green}{a_n}x_{n-1} +\textcolor{red}{b_n}  $

\item \begin{minipage}[t]{0.49\textwidth}$\pi_n = \prod_{i=2}^n\textcolor{green}{a_i}$
\textcolor{gray}{\\Hinweis: $\prod_{i=2}^n3 = 3^{n-1}$
\\\textcolor{white}{Hinweis: }$\prod_{i=2}^ni = n!$}
\mathitem{ x_n =\pi_n\left(\textcolor{blue}{b}+ \sum_{i=2}^n\dfrac{\textcolor{red}{b_{\textbf{i}}} }{\pi_{\textbf{i}}} \right)          }
\end{minipage}
\begin{minipage}[t]{0.49\textwidth}
Einfache Sonderfalle:          
\begin{itemize}
\mathitem{x_n= a_n x_{n-1} =~~~ b \prod_{i=2}^n a_i          }
\mathitem{x_n= x_{n-1} + b_n  = ~~ b + \sum_{i=2}^n b_i     }
\end{itemize}
\end{minipage}
\end{enumerate}
}

\minmeth{Nützliche Zahlen}\\
\halfpage{
\begin{itemize}
\mathitem{ \IN \frac{1}{i} = H_n~~~~\textcolor{lightgray}{Abschatzung: ln(n+1) \leq H_n \leq ln(n)+1         } \\
\IN H_i = (n+1) H_n -n          }


\mathitem{ x_n = \textcolor{red}{\sum_{i=1}^{n-1} x_i} + sth_n \textcolor{lightgray}{\Rightarrow x_{n-1} = \sum_{i=1}^{n-2} x_i + sth_{n-1} \Rightarrow \sum_{i=1}^{n-2} x_i = x_{n-1} - sth_{n-1}} \\ \Rightarrow x_n = 2x_{n-1} +sth_n - sth_{n-1} } 

\item  $\IN c= nc $ \\
\quarterpage{ $\IN i = \frac{n(n+1)}{2}          \\
\IN (2i -1) = n^2$          }
\quarterpage{$ \IN i^2 = \frac{n(n+1)(n+2)}{6}          \\
\IN i^3 = \left( \frac{n(n+1)}{2} \right) ^2          $}

\mathitem{\IN \lfloor log_2(i) \rfloor  = (n+1) \lfloor log_2(n) \rfloor - 2\left( 2^{\lfloor log_2(n) \rfloor} -1 \right)        }

\mathitem{

\geo c^i = \frac{c^{n+1}-1}{c-1}\\
\geo i c^{i-1} = \frac{(n+1)c^n(c-1)-(c^{n+1}-1)}{(c-1)^2}
\sum_{i=2}^n \left( \dfrac{1}{2^{i-1}} \right)  = \sum_i={2^n} \left( \dfrac{1}{2}^{i-1} \right)
}
\end{itemize}
}

\minmeth{rationale Summen}\\
\halfpage{
\begin{enumerate}
\mathitem{\IN \frac{sth}{polynom}}
\mathitem{Partialbruchzerlegung: \frac{x_i}{polynom} = \frac{a}{1.NST} + \frac{b}{2.NST} \dots \\ }
Bei Mehrfachen NST $(k.NST)^{Vielfachheit}$ statt k. NST 
\item Koeffizientenvergleich;
\end{enumerate}}




\newcommand{\tab}{\textcolor{white}{xxx}}
\minmeth{Indexverschiebung}
$\sum_{i=1}^ni-1 = \sum_{i=0}^{n-1} i$\\
\tab \tab \tab \tab \tab \tab $\sum_{i=2}^n i = \sum_{i=0}^{n}(i) -1 -0$


\minmeth{Gleichung erstellen}\\
\tab \halfpage{
for i=1 to n-1 \textbf{\{}\\
\tab DoRec(i)  $\Rightarrow \sum_{i=1}^{n-1}x_i$  // siehe Nützliche Zahlen (rot) \\
\tab DoRec(n-1)  $\Rightarrow  \textcolor{lightgray}{\sum_{i=1}^{n-1}x_{n-1}} = (n-1) x_{n-1}$\\
\tab print("hallo") $\Rightarrow \sum_{i=1}^{n-1}1 = n-1$  
\textbf{\}}
}